don't rely on uint_t/array_t type aliases for record predicate derivation
to avoid ending up with
(@length (uint_t 32) mylist) and
(@length Z mylist)
which aren't recognized as equal by lia

bedrock2/src/bedrock2/RecordPredicates.v
@@ -1,171 +1,70 @@
 Require Import Coq.ZArith.ZArith.
 Require Import coqutil.Word.Interface coqutil.Word.Bitwidth.
 Require Import coqutil.Map.Interface.
-Require Import coqutil.Tactics.RecordEta.
+Require Import coqutil.Tactics.ltac_list_ops.
 Require Import coqutil.Tactics.Tactics.
 Require Import bedrock2.Map.Separation.
 Require Import bedrock2.SepLib.
 Require Export bedrock2.sepapp.
 
-(* Note: Not using a Section here because `Hint Extern` declared inside a Section cannot
-   be exported) *)
+Inductive record_field_description{width: Z}{BW: Bitwidth width}{word: word.word width}
+  {mem: map.map word Byte.byte}(R: Type): Type :=
+| mk_record_field_description(F: Type)(getter: R -> F)(pred: F -> word -> mem -> Prop).
 
-Definition RepPredicate{width: Z}{BW: Bitwidth width}{word: word.word width}
-  {mem: map.map word Byte.byte}(T: Type) := T -> word -> mem -> Prop.
-Existing Class RepPredicate.
+Arguments mk_record_field_description{width}{BW}{word}{mem}{R}{F}.
 
-#[export] Hint Extern 1 (RepPredicate (uint_t ?nbits)) =>
-  exact (uint nbits) : typeclass_instances.
+(* Given a record_field_description for some type R and a variable r of type R,
+   looks up the size of that record field (might depend on r) using typeclass search,
+   and returns it as a sized_predicate *)
+Ltac infer_size r descr :=
+  lazymatch descr with
+  | mk_record_field_description ?getter ?pred =>
+      constr:(mk_sized_predicate (pred (getter r)) _)
+  end.
 
-#[export] Hint Extern 1 (RepPredicate (array_t ?T ?n)) =>
-  match constr:(_: RepPredicate T) with
-  | ?elem => exact (array elem n)
-  end
-: typeclass_instances.
-
-#[export] Hint Extern 1 (RepPredicate (@word.rep ?width ?word)) =>
-  exact (@uintptr width _ word _) : typeclass_instances.
-
-Goal forall width (BW: Bitwidth width) (word: word width) (mem: map.map word Byte.byte)
-            (n: Z),
-  RepPredicate (array_t word n).
-  intros. typeclasses eauto.
-Abort.
-
-Ltac create_predicate_rec refine_already_introd :=
+Ltac create_predicate fields :=
   lazymatch goal with
-  | |- forall (lastField: ?T), ?wo -> ?mem -> Prop =>
-      let f := fresh lastField in
-      intro f;
-      refine (sepapps _);
-      refine_already_introd;
-      match constr:(_ : RepPredicate T) with
-      | ?p => exact (cons (mk_sized_predicate (p f) _) nil)
-      end
-  | |- forall (name: ?T), _ =>
-      let f := fresh name in
-      intro f;
-      match constr:(_ : RepPredicate T) with
-      | ?p => create_predicate_rec
-                ltac:(refine_already_introd; refine (cons (mk_sized_predicate (p f) _) _))
-      end
+  | r: _ |- @word.rep _ _ -> @map.rep _ _ _ -> Prop =>
+      let res := map_with_ltac ltac:(infer_size r) fields in
+      exact (sepapps res)
   end.
-
-(* Given a match expression of the form
-   (match r with {| field1 := x1; ... fieldN := xn |} => body end),
-   returns a proof that this expression equals
-   body[field1 r/x1, ... fieldN r/xn] *)
-Ltac replace_match_by_projections_proof m :=
-  lazymatch m with
-  | (match ?d with _ => _ end) =>
-      let r := reconstruct_record d in
-      constr:(ltac:(replace d with r at 1 by (destruct d; reflexivity); reflexivity)
-               : m = _)
-  end.
-
-Ltac create_predicate :=
-  let G := lazymatch goal with |- ?G => G end in
-  let t := constr:(ltac:(
-             let p := fresh in intro p; case p; create_predicate_rec idtac) : G) in
-  lazymatch constr:(ltac:(
-    let p := fresh in intro p;
-    let m := eval cbv beta in (t p) in
-    let pf := replace_match_by_projections_proof m in
-    lazymatch type of pf with
-    | m = ?m' => exact m'
-    end))
-  with ?x => exact x end.
 
 #[export] Hint Extern 20 (PredicateSize ?p) =>
   let h := head p in unfold h; typeclasses eauto
 : typeclass_instances.
 
-Ltac is_ground_Z x :=
-  lazymatch x with
-  | ?op ?a ?b =>
-      lazymatch (lazymatch op with
-                 | Z.add => constr:(true)
-                 | Z.mul => constr:(true)
-                 | _ => constr:(false)
-                 end) with
-      | true => lazymatch is_ground_Z a with
-                | true => lazymatch is_ground_Z b with
-                          | true => constr:(true)
-                          | false => constr:(false)
-                          end
-                | false => constr:(false)
-                end
-      | false => constr:(false)
-      end
-  | _ => isZcst x
-  end.
-
-Ltac sized_predicate_list_size l :=
-  lazymatch l with
-  | cons (mk_sized_predicate _ ?sz) nil => sz
-  | cons (mk_sized_predicate _ ?sz) ?rest =>
-      let sz' := sized_predicate_list_size rest in
-      constr:(Z.add sz sz')
-  | nil => Z0
-  end.
-
-(* Often, only the last field of a record is of variable size,
-   so computing the size left-associatively and adding up all
-   the constant sizes can simplify the expressions *)
-Ltac sepapps_size_with_ground_acc acc l :=
-  lazymatch l with
-  | cons (mk_sized_predicate _ ?sz) ?rest =>
-      lazymatch is_ground_Z sz with
-      | true => let acc' := eval cbv in (Z.add acc sz) in
-                  sepapps_size_with_ground_acc acc' rest
-      | false => lazymatch sized_predicate_list_size rest with
-                 | Z0 => constr:(Z.add acc sz)
-                 | ?sz' => constr:(Z.add acc (Z.add sz sz'))
-                 end
-      end
-  | nil => acc
-  end.
-
-#[export] Hint Extern 1 (PredicateSize (sepapps ?l)) =>
-  let sz := sepapps_size_with_ground_acc Z0 l in exact sz
-: typeclass_instances.
+(* TODO replace by a notation that looks like C struct definitions *)
+Notation "'record!' fields" := ltac:(create_predicate fields)
+  (at level 10, only parsing).
 
 Module Examples_TODO_move.
-
-  Definition MAC := array_t (uint_t 8) 6.
-  #[export] Hint Extern 1 (RepPredicate MAC) =>
-     exact (array (uint 8) 6) : typeclass_instances.
-
-  Definition IPv4 := array_t (uint_t 8) 4.
-  #[export] Hint Extern 1 (RepPredicate IPv4) =>
-    exact (array (uint 8) 4) : typeclass_instances.
 
   Definition ARPOperationRequest: Z := 1.
   Definition ARPOperationReply: Z := 2.
 
   Record ARPPacket_t := mkARPPacket {
-    htype: uint_t 16; (* hardware type *)
-    ptype: uint_t 16; (* protocol type *)
-    hlen: uint_t 8;   (* hardware address length (6 for MAC addresses) *)
-    plen: uint_t 8;   (* protocol address length (4 for IPv4 addresses) *)
-    oper: uint_t 16;
-    sha: MAC;  (* sender hardware address *)
-    spa: IPv4; (* sender protocol address *)
-    tha: MAC;  (* target hardware address *)
-    tpa: IPv4; (* target protocol address *)
+    htype: Z; (* hardware type *)
+    ptype: Z; (* protocol type *)
+    hlen: Z;  (* hardware address length (6 for MAC addresses) *)
+    plen: Z;  (* protocol address length (4 for IPv4 addresses) *)
+    oper: Z;
+    sha: list Z; (* sender hardware address *)
+    spa: list Z; (* sender protocol address *)
+    tha: list Z; (* target hardware address *)
+    tpa: list Z; (* target protocol address *)
   }.
 
   Record EthernetHeader_t := mkEthernetHeader {
-    dstMAC: MAC;
-    srcMAC: MAC;
-    etherType: uint_t 16;
+    dstMAC: list Z;
+    srcMAC: list Z;
+    etherType: Z;
   }.
 
   Record var_size_foo_t := {
-    foo_size: uint_t 32;
-    foo_stuff: uint_t 16;
-    foo_payload: array_t (uint_t 8) foo_size;
-    foo_trailer: uint_t 16;
+    foo_size: Z;
+    foo_stuff: Z;
+    foo_payload: list Z;
+    foo_trailer: Z;
   }.
 
   Section WithMem.
@@ -173,32 +72,44 @@ Module Examples_TODO_move.
     Context {width: Z} {BW: Bitwidth width} {word: word.word width} {word_ok: word.ok word}.
     Context {mem: map.map word Byte.byte} {mem_ok: map.ok mem}.
 
-    Instance ARPPacket: RepPredicate ARPPacket_t :=
-      ltac:(create_predicate).
+    Definition ARPPacket(r: ARPPacket_t): word -> mem -> Prop := record!
+      (cons (mk_record_field_description htype (uint 16))
+      (cons (mk_record_field_description ptype (uint 16))
+      (cons (mk_record_field_description hlen (uint 8))
+      (cons (mk_record_field_description plen (uint 8))
+      (cons (mk_record_field_description oper (uint 16))
+      (cons (mk_record_field_description sha (array (uint 8) 6))
+      (cons (mk_record_field_description spa (array (uint 8) 4))
+      (cons (mk_record_field_description tha (array (uint 8) 6))
+      (cons (mk_record_field_description tpa (array (uint 8) 4)) nil))))))))).
 
     Goal forall p, (_ : PredicateSize (ARPPacket p)) = 28. intros. reflexivity. Abort.
 
-    Instance EthernetHeader: RepPredicate EthernetHeader_t :=
-      ltac:(create_predicate).
+    Definition EthernetHeader(r: EthernetHeader_t): word -> mem -> Prop := record!
+      (cons (mk_record_field_description dstMAC (array (uint 8) 6))
+      (cons (mk_record_field_description srcMAC (array (uint 8) 6))
+      (cons (mk_record_field_description etherType (uint 16)) nil))).
 
     Goal forall p, (_ : PredicateSize (EthernetHeader p)) = 14. intros. reflexivity. Abort.
 
-    Instance var_size_foo: RepPredicate var_size_foo_t :=
-      ltac:(create_predicate).
+    Definition var_size_foo(r: var_size_foo_t): word -> mem -> Prop := record!
+      (cons (mk_record_field_description foo_size (uint 32))
+      (cons (mk_record_field_description foo_stuff (uint 16))
+      (cons (mk_record_field_description foo_payload (array (uint 8) (foo_size r)))
+      (cons (mk_record_field_description foo_trailer (uint 16)) nil)))).
 
     Goal forall p, (_ : PredicateSize (var_size_foo p)) = 6 + (foo_size p * 1 + 2).
     Proof. intros. reflexivity. Abort.
 
     (* not a Lemma because this kind of goal will be solved inline by sepcalls canceler *)
-    Goal forall (bs: list (uint_t 8)) (R: mem -> Prop) a m (Rest: EthernetHeader_t -> Prop),
+    Goal forall (bs: list Z) (R: mem -> Prop) a m (Rest: EthernetHeader_t -> Prop),
         sep (array (uint 8) 14 bs a) R m ->
         exists h, sep (EthernetHeader h a) R m /\ Rest h.
     Proof.
       intros.
       eexists (mkEthernetHeader _ _ _).
       unfold EthernetHeader.
-      unfold sepapp.
+      cbn.
     Abort.
-
   End WithMem.
 End Examples_TODO_move.
