LiveVerif/src/LiveVerif/LiveVerifLib.v
@@ -1,4 +1,5 @@
 Require Export Coq.ZArith.ZArith. Local Open Scope Z_scope.
+Require Export Coq.micromega.Lia.
 Require Export coqutil.Datatypes.Inhabited.
 Require Export coqutil.Tactics.Tactics.
 Require Export coqutil.Map.Interface coqutil.Map.Properties.
