LiveVerif/src/LiveVerifExamples/ErrorTests/find_superrange_hyp_errors.v
@@ -5,15 +5,19 @@ Ltac pose_err e ::= pose_err_silent e.
 
 Load LiveVerif.
 
-Record bar_t{n: Z} := {
-  barA: uint_t 16;
-  barB: uint_t 16;
+Record bar_t := {
+  barA: Z;
+  barB: Z;
   barC: word;
-  barPayload: array_t (uint_t 32) n;
+  barPayload: list Z;
 }.
 Arguments bar_t: clear implicits.
 
-Instance bar(n: uint_t 32): RepPredicate (bar_t n) := ltac:(create_predicate).
+Definition bar(n: Z)(b: bar_t): word -> mem -> Prop := record!
+  (cons (mk_record_field_description barA (uint 16))
+  (cons (mk_record_field_description barB (uint 16))
+  (cons (mk_record_field_description barC uintptr)
+  (cons (mk_record_field_description barPayload (array (uint 32) n)) nil)))).
 
 #[export] Instance spec_of_swap_barAB: fnspec :=                                .**/
 
