LiveVerif/src/LiveVerifExamples/swap_subarrays.v
@@ -8,7 +8,7 @@ Axiom TODO: False.
 #[export] Instance spec_of_swap_16s: fnspec :=                                  .**/
 
 void swap_16s(uintptr_t p1, uintptr_t p2, uintptr_t n) /**#
-  ghost_args := (l1 l2: list (uint_t 16)) (R: mem -> Prop);
+  ghost_args := (l1 l2: list Z) (R: mem -> Prop);
   requires t m := <{ * array (uint 16) \[n] l1 p1
                      * array (uint 16) \[n] l2 p2
                      * R }> m;
@@ -24,7 +24,7 @@ Qed.
 #[export] Instance spec_of_swap_subarrays: fnspec :=                            .**/
 
 void swap_subarrays(uintptr_t p, uintptr_t i, uintptr_t j, uintptr_t count) /**#
-  ghost_args := (l: list (uint_t 16)) n (R: mem -> Prop);
+  ghost_args := (l: list Z) n (R: mem -> Prop);
   requires t m :=
       \[i] + \[count] <= \[j] /\
       \[j] + \[count] <= n /\
@@ -37,9 +37,8 @@ Derive swap_subarrays SuchThat (fun_correct! swap_subarrays) As
   swap_subarrays_ok.                                                            .**/
 {                                                                          /**. .**/
   swap_16s(p + 2 * i, p + 2 * j, count);                                   /**.
-
   Unshelve.
-all: case TODO.
+  all: case TODO.
 Qed.
 
 End LiveVerif. Comments .**/ //.
