bedrock2/src/bedrock2/sepapp.v
@@ -187,3 +187,53 @@ Section Reassociate_sepapp.
 End Reassociate_sepapp.
 
 #[export] Hint Resolve purify_sepapps: purify.
+
+Ltac is_ground_Z x :=
+  lazymatch x with
+  | ?op ?a ?b =>
+      lazymatch (lazymatch op with
+                 | Z.add => constr:(true)
+                 | Z.mul => constr:(true)
+                 | _ => constr:(false)
+                 end) with
+      | true => lazymatch is_ground_Z a with
+                | true => lazymatch is_ground_Z b with
+                          | true => constr:(true)
+                          | false => constr:(false)
+                          end
+                | false => constr:(false)
+                end
+      | false => constr:(false)
+      end
+  | _ => isZcst x
+  end.
+
+Ltac sized_predicate_list_size l :=
+  lazymatch l with
+  | cons (mk_sized_predicate _ ?sz) nil => sz
+  | cons (mk_sized_predicate _ ?sz) ?rest =>
+      let sz' := sized_predicate_list_size rest in
+      constr:(Z.add sz sz')
+  | nil => Z0
+  end.
+
+(* Often, only the last field of a record is of variable size,
+   so computing the size left-associatively and adding up all
+   the constant sizes can simplify the expressions *)
+Ltac sepapps_size_with_ground_acc acc l :=
+  lazymatch l with
+  | cons (mk_sized_predicate _ ?sz) ?rest =>
+      lazymatch is_ground_Z sz with
+      | true => let acc' := eval cbv in (Z.add acc sz) in
+                  sepapps_size_with_ground_acc acc' rest
+      | false => lazymatch sized_predicate_list_size rest with
+                 | Z0 => constr:(Z.add acc sz)
+                 | ?sz' => constr:(Z.add acc (Z.add sz sz'))
+                 end
+      end
+  | nil => acc
+  end.
+
+#[export] Hint Extern 1 (PredicateSize (sepapps ?l)) =>
+  let sz := sepapps_size_with_ground_acc Z0 l in exact sz
+: typeclass_instances.
